theories/logrel/stlc/lang.v
@@ -77,22 +77,22 @@ Module stlc.
 
   Definition state : Type := ().
 
-  Inductive head_step : expr → state → list Empty_set → expr → state → list expr → Prop :=
+  Inductive base_step : expr → state → list Empty_set → expr → state → list expr → Prop :=
   | BetaS e1 e2 v2 σ :
       to_val e2 = Some v2 →
-      head_step (App (Lam e1) e2) σ [] e1.[e2/] σ []
+      base_step (App (Lam e1) e2) σ [] e1.[e2/] σ []
   | FstS e1 v1 e2 v2 σ :
       to_val e1 = Some v1 → to_val e2 = Some v2 →
-      head_step (Fst (Pair e1 e2)) σ [] e1 σ []
+      base_step (Fst (Pair e1 e2)) σ [] e1 σ []
   | SndS e1 v1 e2 v2 σ :
       to_val e1 = Some v1 → to_val e2 = Some v2 →
-      head_step (Snd (Pair e1 e2)) σ [] e2 σ []
+      base_step (Snd (Pair e1 e2)) σ [] e2 σ []
   | CaseLS e0 v0 e1 e2 σ :
       to_val e0 = Some v0 →
-      head_step (Case (InjL e0) e1 e2) σ [] e1.[e0/] σ []
+      base_step (Case (InjL e0) e1 e2) σ [] e1.[e0/] σ []
   | CaseRS e0 v0 e1 e2 σ :
       to_val e0 = Some v0 →
-      head_step (Case (InjR e0) e1 e2) σ [] e2.[e0/] σ [].
+      base_step (Case (InjR e0) e1 e2) σ [] e2.[e0/] σ [].
 
   (** Basic properties about the language *)
   Lemma to_of_val v : to_val (of_val v) = Some v.
@@ -114,11 +114,11 @@ Module stlc.
   Proof. destruct Ki; intros ???; simplify_eq; auto with f_equal. Qed.
 
   Lemma val_stuck e1 σ1 κ e2 σ2 ef :
-    head_step e1 σ1 κ e2 σ2 ef → to_val e1 = None.
+    base_step e1 σ1 κ e2 σ2 ef → to_val e1 = None.
   Proof. destruct 1; naive_solver. Qed.
 
-  Lemma head_ctx_step_val Ki e σ1 κ e2 σ2 ef :
-    head_step (fill_item Ki e) σ1 κ e2 σ2 ef → is_Some (to_val e).
+  Lemma base_ctx_step_val Ki e σ1 κ e2 σ2 ef :
+    base_step (fill_item Ki e) σ1 κ e2 σ2 ef → is_Some (to_val e).
   Proof. destruct Ki; inversion_clear 1; simplify_option_eq; eauto. Qed.
 
   Lemma fill_item_no_val_inj Ki1 Ki2 e1 e2 :
@@ -131,13 +131,13 @@ Module stlc.
            end; auto.
   Qed.
 
-  Lemma val_head_stuck e1 σ1 κ e2 σ2 efs : head_step e1 σ1 κ e2 σ2 efs → to_val e1 = None.
+  Lemma val_base_stuck e1 σ1 κ e2 σ2 efs : base_step e1 σ1 κ e2 σ2 efs → to_val e1 = None.
   Proof. destruct 1; naive_solver. Qed.
 
-  Lemma lang_mixin : EctxiLanguageMixin of_val to_val fill_item head_step.
+  Lemma lang_mixin : EctxiLanguageMixin of_val to_val fill_item base_step.
   Proof.
-    split; apply _ || eauto using to_of_val, of_to_val, val_head_stuck,
-           fill_item_val, fill_item_no_val_inj, head_ctx_step_val.
+    split; apply _ || eauto using to_of_val, of_to_val, val_base_stuck,
+           fill_item_val, fill_item_no_val_inj, base_ctx_step_val.
   Qed.
 End stlc.
 
