theories/concurrent_stacks/concurrent_stack4.v
@@ -289,7 +289,7 @@ Section proofs.
   Proof.
     destruct xs; first by iIntros "? %".
     iIntros "Hl Hstack"; iDestruct "Hstack" as (t') "(Hl' & Hrest)".
-    iDestruct (mapsto_agree with "Hl Hl'") as "%"; simplify_eq; iExists _; auto.
+    iDestruct (pointsto_agree with "Hl Hl'") as "%"; simplify_eq; iExists _; auto.
   Qed.
 
   Definition stack_inv P l :=
@@ -335,7 +335,7 @@ Section proofs.
       iInv Nstack as (list' xs) "(Hl & Hlist & HP)" "Hclose".
       destruct (decide (list = list')) as [ -> |].
       * wp_cmpxchg_suc. { destruct list'; left; done. }
-        iMod (mapsto_persist with "Hl'") as "#Hl'".
+        iMod (pointsto_persist with "Hl'") as "#Hl'".
         iMod (fupd_mask_subseteq inner_mask) as "Hupd'"; first solve_ndisj.
         iMod ("Hupd" with "HP") as "[HP HΨ]".
         iMod "Hupd'" as "_".
@@ -418,7 +418,7 @@ Section proofs.
           iMod ("Hupdcons" with "HP") as "[HP HΨ]".
           iMod "Hupd'" as "_".
           iDestruct "Hlist" as (t') "(Hl'' & Hlist)".
-          iDestruct (mapsto_agree with "Hl' Hl''") as "%"; simplify_eq.
+          iDestruct (pointsto_agree with "Hl' Hl''") as "%"; simplify_eq.
           iMod ("Hclose" with "[Hlist Hl HP]") as "_".
           { iNext; iExists _, _; iFrame. }
           iModIntro.
